src/prototype/Min.v
@@ -1,0 +1,40 @@
+Require Import Vector.
+Import Vector.VectorNotations.
+Require Import Program.Equality.
+Require Import Coq.Program.Wf.
+From Hammer Require Import Tactics.
+From Hammer Require Import Hammer.
+Require Import Lia.
+Inductive instr1 : Type := | A : instr1 | B : instr1.
+Inductive instr2 : Type := | A' : instr2 | B' : instr2 | C' : instr2.
+Fixpoint comp_len {n} (p : t instr1 n) : nat :=
+  match p with
+  | [] => 0
+  | A :: xs => 1 + comp_len xs
+  | B :: xs => 3 + comp_len xs
+  end.
+Fixpoint compile {n} (p : Vector.t instr1 n) : Vector.t instr2 (comp_len p) :=
+  match p with
+  | [] => []
+  | A :: p' => A' :: compile p'
+  | B :: p' => C' :: B' :: A' :: compile p'
+  end.
+Fixpoint compile_index {n} (p : t instr1 n) (x : Fin.t n) : Fin.t (comp_len p).
+Proof.
+  destruct x eqn:H1; rewrite (eta p); destruct hd eqn:H2.
+  - apply Fin.F1.
+  - apply Fin.F1.
+  - do 1 apply Fin.FS. apply compile_index. exact t.
+  - do 3 apply Fin.FS. apply compile_index. exact t.
+Defined.
+Fixpoint to_nat {n} (x : Fin.t n) : nat :=
+  match x with
+  | Fin.F1 => 0
+  | Fin.FS t => 1 + (to_nat t)
+  end.
+
+Theorem th {n} : forall p x x' (off : Fin.t (comp_len [p[@x]])),
+                  to_nat x' = to_nat (@compile_index n p x) + to_nat off ->
+                  (compile p)[@x'] = (compile [p[@x]])[@off].
+
+
